partial correctness proof of monadic `List.findIndex!`

Qsort/Experiments.lean
@@ -2,17 +2,27 @@ import MPL
 
 open MPL
 
-partial def List.findIndex (xs : List α) (p : α → Bool) : EStateM Unit Unit Nat := do
+theorem EStateM.by_wp' {α} {x : EStateM.Result ε σ α} {prog : EStateM ε σ α} (h : EStateM.run prog s = x) (P : EStateM.Result ε σ α → Prop) :
+  ((wp prog).apply (post⟨fun a s' => P (EStateM.Result.ok a s'), fun e s' => P (EStateM.Result.error e s')⟩) s) → P x := by
+  sorry
+    -- intro hspec
+    -- simp [wp, PredTrans.pure] at hspec
+    -- split at hspec
+    -- case h_1 a s' heq => rw[← heq] at hspec; exact h ▸ hspec
+    -- case h_2 => contradiction
+
+partial def List.findIndex! (xs : List α) (p : α → Bool) : EStateM Unit Unit Nat := do
   match xs with
   | [] => throw ()
   | x::ys => do
     if p x then
       pure 0
     else
-      let r ← List.findIndex ys p
+      let r ← List.findIndex! ys p
       pure (r + 1)
 -- partial_fixpoint
-def List.__findIndex (f : (xs : List α) → (p : α → Bool) → EStateM Unit Unit Nat) (xs : List α) (p : α → Bool) : EStateM Unit Unit Nat := do
+
+def List.__findIndex! (f : (xs : List α) → (p : α → Bool) → EStateM Unit Unit Nat) (xs : List α) (p : α → Bool) : EStateM Unit Unit Nat := do
   match xs with
   | [] => throw ()
   | x::ys =>
@@ -22,31 +32,80 @@ def List.__findIndex (f : (xs : List α) → (p : α → Bool) → EStateM Unit 
       let r ← f ys p
       pure (r + 1)
 
-def List.findIndex.partial_correctness (motive : List α → (α → Bool) → _ → Prop)
-  (hf : ∃ f, List.__findIndex f = f)
+def List.__findIndex!.partial_correctness (motive : List α → (α → Bool) → Unit → _ → Prop)
+  (hf : ∃ f, List.__findIndex! f = f)
   (h :
     ∀ (f : List α → (α → Bool) → EStateM Unit Unit Nat),
-      (∀ (xs : List α) (p : α → Bool) (r : _), (f xs p).run () = r → motive xs p r) →
-        ∀ (xs : List α) (p : α → Bool) (r : _),
-          (List.__findIndex f xs p).run () = r →
-            motive xs p r)
-  (xs : List α) (p : α → Bool) (r : _) : (hf.choose xs p).run () = r → motive xs p r := sorry
+      (∀ (xs : List α) (p : α → Bool) (s : Unit) (r : _), (f xs p).run s = r → motive xs p s r) →
+        ∀ (xs : List α) (p : α → Bool) (s : Unit) (r : _),
+          (List.__findIndex! f xs p).run s = r →
+            motive xs p s r)
+  (xs : List α) (p : α → Bool) (s : Unit) (r : _) : (hf.choose xs p).run s = r → motive xs p s r := sorry
 
-theorem List.findIndex_implies_pred
-    (hf : ∃ f, List.__findIndex f = f)
-    (xs : List α) (p : α → Bool) :
-    (hf.choose xs p).run () = r →
-    if let (.ok i _) := r then
-      ∃x, xs[i]? = some x ∧ p x
-    else
-      ∀ (i : Nat) x, xs[i]? = some x → ¬ (p x)
-    := by
-      refine List.findIndex.partial_correctness (fun xs p r => _) hf (fun f ih => ?_) xs p r
-      intros xs p r h
-      apply EStateM.by_wp h
-      sorry
+-- set_option trace.mpl.tactics.spec true in
+theorem List.__findIndex!_implies_pred_triple
+  (xs : List α) (p : α → Bool)
+  (f : List α → (α → Bool) → EStateM Unit Unit Nat)
+  (ih : ∀ (xs : List α) (p : α → Bool),
+    ⦃⌜True⌝⦄
+    f xs p
+    ⦃post⟨fun i _ => ∃x, xs[i]? = some x ∧ p x,
+          fun e s => ∀ (i : Nat) x, xs[i]? = some x → ¬ (p x)⟩⦄)
+  :
+    ⦃⌜True⌝⦄
+    List.__findIndex! f xs p
+    ⦃post⟨fun i _ => ∃x, xs[i]? = some x ∧ p x,
+          fun e s => ∀ (i : Nat) x, xs[i]? = some x → ¬ (p x)⟩⦄ := by
+  simp_all only [Bool.not_eq_true]
+  unfold __findIndex!
+  mintro - ∀s
+  split
+  . mwp
+    simp
+  next y ys =>
+  mwp
+  split
+  . simpa
+  next hn =>
+  simp only [Bool.not_eq_true] at hn
+  mspec ih ys p
+  mintro ∀_
+  mpure h
+  mpure_intro
+  intros i x
+  cases i with
+  | zero =>
+    simp
+    rintro rfl
+    assumption
+  | succ n =>
+    simp
+    have := h n x
+    assumption
+  massumption
+
+theorem List.__findIndex!_implies_pred
+  (hf : ∃ f, List.__findIndex! f = f)
+  (xs : List α) (p : α → Bool) :
+  (hf.choose xs p).run () = r →
+  if let (.ok i _) := r then
+    ∃x, xs[i]? = some x ∧ p x
+  else
+    ∀ (i : Nat) x, xs[i]? = some x → ¬ (p x)
+  := by
+    refine List.__findIndex!.partial_correctness (fun xs p s r => 
+      if let (.ok i _) := r then
+        ∃x, xs[i]? = some x ∧ p x
+      else
+        ∀ (i : Nat) x, xs[i]? = some x → ¬ (p x)
+      ) hf (fun f ih => ?_) xs p () r
+    intros xs p s r h
+    apply EStateM.by_wp' h
+    refine List.__findIndex!_implies_pred_triple xs p f (fun xs p s => ?_) s True.intro
+    refine fun _ => ?_
+    simp only [wp] ; split <;> next h => exact ih xs p _ _ h
 
 -- #print List.findIndex
 -- #print List.findIndex.partial_correctness
 --
-#eval (List.findIndex ["a", "b", "c"] fun s => s == "b").run ()
+#eval (List.findIndex! ["a", "b", "c"] fun s => s == "b").run ()
